theories/clang/lib/spawn.v
@@ -1,0 +1,1 @@
+From iris_c.clang Require Import logic notations tactics.
